proof/spec/KyberLib.ec
@@ -1,7 +1,7 @@
 require import AllCore IntDiv FloorCeil StdOrder RealExp List.
 require import ZModP Ring.
 require import Distr DList DistrExtra DMap DInterval.
-require import PKE_Ext.
+require import PKE_ROM.
 from Jasmin require import JWord JUtils.
 require import Array25 Array32 Array34 Array64 Array128 Array168 Array256 Array384.
 require import Array768 Array960 Array1024 Array1088 Array1184 Array1152.
